veric/semax_ext.v
@@ -1,0 +1,304 @@
+Require Import veric.base.
+Require Import msl.rmaps.
+Require Import veric.compcert_rmaps.
+Import Mem.
+Require Import msl.msl_standard.
+Require Import veric.juicy_mem veric.juicy_mem_lemmas veric.juicy_mem_ops.
+Require Import sepcomp.extspec.
+Require Import veric.juicy_extspec.
+Require Import veric.expr. 
+Require Import veric.semax.
+
+Definition funsig2signature (s : funsig) : signature :=
+  mksignature (map typ_of_type (map snd (fst s))) (Some (typ_of_type (snd s))) cc_default.
+
+Definition ef_id ef :=
+  match ef with EF_external id sig => id | _ => 1%positive end.
+
+Section funspecs2jspec.
+
+Variable Z : Type.
+
+Variable Espec : juicy_ext_spec Z.
+
+Variable gx : genv.
+
+Definition funspec2types id (A : Type) (ef : external_function) : Type :=
+  if ident_eq id (ef_id ef) then A else (ext_spec_type Espec ef).
+
+Definition funspec2pre (A : Type) P id ef x (tys : list typ) args (z : Z) m : Prop :=
+  match ident_eq id (ef_id ef) as s 
+  return ((if s then A else ext_spec_type Espec ef) -> Prop)
+  with 
+    | left _ => fun x' => P x' (make_ext_args gx 1 args) (m_phi m)
+    | right n => fun x' => ext_spec_pre Espec ef x' tys args z m
+  end x.
+
+Definition funspec2post (A : Type) Q id ef x (tret : option typ) ret (z : Z) m : Prop :=
+  match ident_eq id (ef_id ef) as s 
+  return ((if s then A else ext_spec_type Espec ef) -> Prop)
+  with 
+    | left _ => fun x' => Q x' (make_ext_rval 1 ret) (m_phi m)
+    | right n => fun x' => ext_spec_post Espec ef x' tret ret z m
+  end x.
+
+Definition funspec2extspec (f : (ident*funspec)) 
+  : external_specification juicy_mem external_function Z :=
+  match f with 
+    | (id, mk_funspec sig A P Q) =>
+      Build_external_specification juicy_mem external_function Z
+        (fun ef => if ident_eq id (ef_id ef) then A else ext_spec_type Espec ef)
+        (funspec2pre A P id)
+        (funspec2post A Q id)
+        (fun rv z m => False)
+  end.
+
+Definition wf_funspec (f : funspec) :=
+  match f with
+    | mk_funspec sig A P Q => 
+      forall a rho rho' phi phi', 
+        P a rho phi -> Q a rho' phi' -> 
+        (level phi' < level phi)%nat 
+        /\ (forall adr, 
+            match phi @ adr with
+              | NO _ => True
+              | YES _ _ _ _ => True
+              | PURE _ _ => phi @ adr = phi' @ adr
+            end)
+  end.
+
+Program Definition funspec2jspec f (wf : wf_funspec (snd f)) : juicy_ext_spec Z :=
+  Build_juicy_ext_spec _ (funspec2extspec f) 
+    _ _ _
+    (fun jm jm' => 
+       (level jm' < level jm)%nat /\ pures_sub jm jm'
+       \/ JE_R _ Espec jm jm')
+    _ _.
+Next Obligation.
+destruct f; simpl; unfold funspec2pre; simpl.
+simpl in t; revert t.
+destruct (ident_eq i (ef_id e)).
+* clear wf; subst i; intros t a a' Hage; destruct m; simpl.
+solve[apply h; apply age_jm_phi; auto].
+* intros ? ? ?; auto.
+destruct Espec; simpl; apply JE_pre_hered.
+Qed.
+Next Obligation.
+destruct f; simpl; unfold funspec2post; simpl.
+simpl in t; revert t.
+destruct (ident_eq i (ef_id e)).
+* clear wf; subst i; intros t a a' Hage; destruct m0; simpl.
+apply h; apply age_jm_phi; auto.
+* intros ? ? ?; auto.
+destruct Espec; simpl; apply JE_post_hered.
+Qed.
+Next Obligation.
+intros ? ? ? ?; destruct f; auto.
+Qed.
+Next Obligation.
+destruct H; auto.
+apply (JE_Rprop _ Espec); auto.
+Qed.
+Next Obligation.
+destruct f; unfold jspec_rel; simpl; intros.
+revert wf; unfold wf_funspec; simpl; intros H2. revert t H H0 H2. 
+unfold funspec2pre, funspec2post. 
+destruct (ident_eq i (ef_id e)).
+* intros.
+specialize (H2 t (make_ext_args gx 1 args) (make_ext_rval 1 rv)). 
+specialize (H2 (m_phi jm) (m_phi jm') H H0).
+destruct H2; auto.
+* destruct Espec; simpl; intros.
+clear H2; right; eapply (JE_rel e); eauto.
+Qed.
+
+End funspecs2jspec.
+
+Inductive wf_funspecs := 
+| wf_nil : wf_funspecs
+| wf_cons : forall (f : ident*funspec) (wf : wf_funspec (snd f)) (l : wf_funspecs), 
+              wf_funspecs.
+
+Fixpoint in_funspecs (f : (ident*funspec)) (fs : wf_funspecs) :=
+  match fs with
+    | wf_nil => False
+    | wf_cons f' wf fs' => f=f' \/ in_funspecs f fs'
+  end.
+
+Fixpoint in_funspecs_by_id (f : (ident*funspec)) (fs : wf_funspecs) :=
+  match fs with
+    | wf_nil => False
+    | wf_cons f' wf fs' => fst f=fst f' \/ in_funspecs_by_id f fs'
+  end.
+
+Lemma in_funspecs_by_id_lem id f f' fs : 
+  in_funspecs_by_id (id,f) fs <-> in_funspecs_by_id (id,f') fs.
+Proof.
+elim fs; simpl; [split; auto|].
+intros [? ?]; simpl; intros H H2 H3; rewrite H3; split; auto.
+Qed.
+
+Lemma in_funspecs_in_by_id f fs :
+  in_funspecs f fs -> 
+  in_funspecs_by_id f fs.
+Proof.
+elim fs; simpl; auto.
+intros [? ?]; simpl; intros ? ? IH.
+intros [?|?]. subst. left; auto. right; auto.
+Qed.
+
+Fixpoint funspecs_norepeat fs :=
+  match fs with
+    | wf_nil => True
+    | wf_cons f wf fs' => ~in_funspecs_by_id f fs' /\ funspecs_norepeat fs'
+  end.
+
+Lemma in_funspecs_wf f fs : in_funspecs f fs -> wf_funspec (snd f).
+Proof. induction fs; simpl; inversion 1; try subst f0; auto. Qed.
+
+Fixpoint add_funspecs_rec (Z : Type) (Espec : juicy_ext_spec Z) gx (fs : wf_funspecs) :=
+  match fs with
+    | wf_nil => Espec
+    | wf_cons (i,f) wf fs' => funspec2jspec Z (add_funspecs_rec Z Espec gx fs') gx (i,f) wf
+  end.
+
+Require Import JMeq.
+
+Lemma add_funspecs_pre {Z gx fs id sig A P Q x args m} Espec tys :
+  let ef := EF_external id (funsig2signature sig) in
+  funspecs_norepeat fs -> 
+  in_funspecs (id, (mk_funspec sig A P Q)) fs -> 
+  P x (make_ext_args gx 1%positive args) (m_phi m) ->
+  exists x' : ext_spec_type (JE_spec _ (add_funspecs_rec Z Espec gx fs)) ef, 
+    JMeq x x' /\ forall z, ext_spec_pre (add_funspecs_rec Z Espec gx fs) ef x' tys args z m.
+Proof.
+induction fs; [intros; elimtype False; auto|]; intros ef H H1 H2.
+destruct H1 as [H1|H1].
+
+{ 
+subst f;simpl in *.
+clear IHfs H; revert x H2; unfold funspec2pre; simpl.
+destruct (ident_eq id id); simpl.
+solve[intros x Hp; exists x; auto].
+solve[elimtype False; auto]. 
+}
+
+{ 
+assert (Hin: in_funspecs_by_id (id, mk_funspec sig A P Q) fs). 
+{ clear -H1; apply in_funspecs_in_by_id in H1; auto. }
+destruct H as [Ha Hb]. 
+destruct (IHfs Hb H1 H2) as [x' H3].
+clear -Ha Hin H1 H3; revert x' Ha Hin H1 H3.
+destruct f; simpl; destruct f; simpl; unfold funspec2pre; simpl.
+destruct (ident_eq i id).
+* subst i; destruct fs; [solve[simpl; intros; elimtype False; auto]|].
+  intros x' Ha Hb; simpl in Ha, Hb.
+  rewrite in_funspecs_by_id_lem with (f' := mk_funspec f A0 m0 m1) in Hb.
+  elimtype False; auto.
+* intros; eexists; eauto.
+}
+Qed.
+
+Lemma add_funspecs_post {Z Espec tret gx fs id sig A P Q x ret m z} :
+  let ef := EF_external id (funsig2signature sig) in
+  funspecs_norepeat fs -> 
+  in_funspecs (id, (mk_funspec sig A P Q)) fs -> 
+  ext_spec_post (add_funspecs_rec Z Espec gx fs) ef x tret ret z m -> 
+  exists x' : A, 
+    JMeq x x' /\ Q x' (make_ext_rval 1%positive ret) (m_phi m).
+Proof.
+induction fs; [intros; elimtype False; auto|]; intros ef H H1 H2.
+destruct H1 as [H1|H1].
+
+{ 
+subst f;simpl in *.
+clear IHfs H; revert x H2; unfold funspec2post; simpl.
+destruct (ident_eq id id); simpl.
+solve[intros x Hp; exists x; auto].
+solve[elimtype False; auto]. 
+}
+
+{ 
+assert (Hin: in_funspecs_by_id (id, mk_funspec sig A P Q) fs). 
+{ clear -H1; apply in_funspecs_in_by_id in H1; auto. }
+destruct H as [Ha Hb]. 
+clear -Ha Hin H1 H2 Hb IHfs; revert x Ha Hin H1 H2 Hb IHfs.
+destruct f; simpl; destruct f; simpl; unfold funspec2post; simpl.
+destruct (ident_eq i id).
+* subst i; destruct fs; [solve[simpl; intros; elimtype False; auto]|].
+  intros x' Ha Hb; simpl in Ha, Hb.
+  rewrite in_funspecs_by_id_lem with (f' := mk_funspec f A0 m0 m1) in Hb.
+  elimtype False; auto.
+* intros. apply IHfs; auto.
+}
+Qed.
+
+Definition add_funspecs (Espec : OracleKind) gx (fs : wf_funspecs) : OracleKind :=
+  match Espec with
+    | Build_OracleKind ty spec => 
+      Build_OracleKind ty (add_funspecs_rec ty spec gx fs)
+  end.
+
+Definition local_funspec (f : funspec) :=
+  match f with mk_funspec spec A P Q => 
+      (* safety monotonicity *)
+      (forall (x : A) rho phi1 phi2 phi, join phi1 phi2 phi -> 
+         P x rho phi1 -> P x rho phi)
+      (* frame property *)
+   /\ (forall (x : A) rho phi1 phi2 phi, join phi1 phi2 phi -> 
+         P x rho phi1 -> 
+       forall rho' phi', (level phi >= level phi')%nat -> 
+         Q x rho' phi' ->
+         exists phi1' phi2', 
+         join phi1' phi2' phi' /\ age phi2 phi2' /\ Q x rho' phi1')         
+  end.
+
+Section semax_ext.
+
+Variable Espec : OracleKind.
+
+(*[NOTE genv]: semax_external should be parameterized by gx. *)
+
+Lemma semax_ext gx id sig A P Q (fs : wf_funspecs) : 
+  let f := mk_funspec sig A P Q in
+  local_funspec f -> 
+  in_funspecs (id,f) fs -> 
+  funspecs_norepeat fs -> 
+  (forall n, semax_external (add_funspecs Espec gx fs) 
+                            (EF_external id (funsig2signature sig)) _ P Q n).
+Proof.
+intros f Hloc Hin Hnorepeat.
+unfold semax_external.
+intros n ge x n0 Hlater F ts args jm H jm' H2 H3.
+destruct H3 as [s [t [Hjoin [Hp Hf]]]].
+cut (P x (make_ext_args ge 1 args) (m_phi jm')). intro Hp'.
+destruct Espec.
+destruct (add_funspecs_pre OK_spec ts Hnorepeat Hin Hp') as [x' [Heq Hpre]].
+simpl.
+assert (ge = gx) as <- by admit. (*cf. [NOTE genv]*)
+exists x'.
+intros z.
+split; [solve[apply Hpre]|].
+intros tret ret z' jm2 Hlev jm3 Hnec Hpost.
+
+cut (Q x (make_ext_rval 1 ret) (m_phi jm3)). intro Hq.
+unfold f in Hloc.
+destruct Hloc as [Hl1 Hl2].
+assert (Hlev': (level (m_phi jm') >= level (m_phi jm3))%nat). 
+{ cut ((level (m_phi jm2) >= level (m_phi jm3))%nat). omega.
+  apply necR_level in Hnec; erewrite <-level_juice_level_phi; eauto. }
+destruct (Hl2 _ _ s t (m_phi jm') Hjoin Hp _ _ Hlev' Hq) 
+  as [phi' [t' [Hjoin' [Hage' Hq']]]].
+exists phi', t'; split; auto.
+split; auto. destruct F. simpl in Hf|-*. eapply h in Hf; eauto.
+
+eapply add_funspecs_post in Hpost; eauto.
+destruct Hpost as [x'' [Heq' Hq']].
+assert (JMeq x x'') by (eapply JMeq_trans; eauto).
+solve[apply JMeq_eq in H1; subst; auto].
+
+unfold f in Hloc; destruct Hloc as [Hloc _]. 
+solve[eapply Hloc; eauto].
+Qed.
+  
+End semax_ext.  
